[lf] wip on logs (needs mono_list straight away).

aneris/examples/reliable_communication/lib/repdb/proof/log_proof.v
@@ -4,15 +4,20 @@ From iris.base_logic Require Import invariants.
 From iris.bi.lib Require Import fractional.
 From iris.proofmode Require Import tactics.
 From aneris.lib Require Import gen_heap_light.
-From aneris.aneris_lang Require Import lang resources inject.
+From aneris.aneris_lang Require Import lang resources inject tactics proofmode.
 From aneris.aneris_lang.lib Require Import
-     list_proof monitor_proof lock_proof map_proof.
+     list_proof monitor_proof lock_proof map_proof assert_proof.
+From aneris.examples.reliable_communication.lib.repdb
+     Require Export log_code.
+From aneris.examples.reliable_communication.lib.repdb.resources
+     Require Import ras resources_def.
+
 Import lock_proof.
 
 
   (* ------------------------------------------------------------------------ *)
   Section Log.
-
+    Context `{!anerisG Mdl Σ, !lockG Σ}.
   Definition inject_log `{!Inject A val} (xs : list A) :=
     ($xs, #(List.length xs))%V.
 
@@ -34,4 +39,202 @@ Import lock_proof.
 
   (* Definition is_logLoc (logM : list A) (logL : loc) : iProp Σ := *)
   (*   ∃ (logV : val), logL ↦[ip] logV ∗ ⌜is_log logM logV⌝. *)
+
+  Lemma wp_log_create ip :
+    {{{ True }}}
+      log_create #() @[ip]
+    {{{ logL logV, RET #logL; logL ↦[ip] logV ∗ ⌜is_log [] logV⌝}}}.
+  Proof.
+    iIntros (Φ) "_ HΦ".
+    wp_rec. wp_pures.
+    wp_alloc l as "Hl".
+    iApply "HΦ". iFrame. iPureIntro.
+    by eexists.
+    Qed.
+
+
+  Lemma wp_log_add_entry ip logL logV logM (x : A) :
+    {{{ ⌜is_log logM logV⌝ ∗ logL ↦[ip] logV }}}
+      log_add_entry #logL $x @[ip]
+    {{{ logV', RET #();
+        ⌜is_log (logM ++ [x]) logV'⌝ ∗ logL ↦[ip] logV' }}}.
+  Proof.
+    iIntros (Φ) "(%Hl & Hp) HΦ".
+    destruct Hl as (lV & -> & Hlst).
+    wp_lam. wp_pures.
+    wp_load. wp_pures.
+    wp_apply (wp_list_cons _ []); first done.
+    iIntros (v) "%Hl2".
+    wp_apply wp_list_append; first done.
+    iIntros (v') "%Hl'".
+    wp_pures.
+    wp_store.
+    iApply "HΦ".
+    iFrame.
+    iPureIntro.
+    eexists; rewrite app_length /=; split; last done.
+    do 3 f_equal; lia.
+  Qed.
+
+
+  Lemma wp_log_next ip logL logV logM q :
+    {{{ ⌜is_log logM logV⌝ ∗ logL ↦[ip]{q} logV }}}
+      log_next #logL @[ip]
+    {{{ n, RET #n;
+        ⌜n = List.length logM⌝ ∗ ⌜is_log (logM) logV⌝ ∗ logL ↦[ip]{q} logV}}}.
+  Proof.
+    iIntros (Φ) "(%Hl & Hp) HΦ".
+    destruct Hl as (lV & -> & Hlst).
+    wp_lam.
+    wp_load.
+    wp_pures.
+    iApply "HΦ".
+    iFrame.
+    iPureIntro.
+    split; by eexists.
+  Qed.
+
+  Lemma wp_log_length ip logL logV logM q :
+    {{{ ⌜is_log logM logV⌝ ∗ logL ↦[ip]{q} logV }}}
+      log_length #logL @[ip]
+    {{{ n, RET #n;
+        ⌜n = List.length logM⌝ ∗ ⌜is_log (logM) logV⌝ ∗ logL ↦[ip]{q} logV}}}.
+  Proof.
+    iIntros (Φ) "(%Hl & Hp) HΦ".
+    destruct Hl as (lV & -> & Hlst).
+    wp_lam.
+    wp_load.
+    wp_pures.
+    iApply "HΦ".
+    iFrame.
+    iPureIntro.
+    split; by eexists.
+  Qed.
+
+Lemma wp_log_get ip logL logV logM i q :
+    {{{ ⌜i < List.length logM⌝ ∗
+        ⌜is_log logM logV⌝ ∗ logL ↦[ip]{q} logV }}}
+      log_get #logL #i @[ip]
+    {{{ x, RET (SOMEV $x);
+        ⌜List.nth_error logM i = Some x⌝ ∗
+        ⌜is_log (logM) logV⌝ ∗ logL ↦[ip]{q} logV}}}.
+  Proof.
+    iIntros (Φ) "(%Hi & %Hl & Hp) HΦ".
+    destruct Hl as (lV & -> & Hlst).
+    wp_lam.
+    wp_pures.
+    wp_load.
+    wp_pures.
+    wp_apply wp_list_nth_some; [eauto with lia|].
+    iIntros (v (x & -> & Hsome)).
+    iApply "HΦ".
+    iFrame.
+    iPureIntro.
+    split; eauto; last by eexists.
+  Qed.
+
+
+  (* Definition logMonitor_res *)
+  (*  ip (γlog : gname) (logL : loc) (Res : list A → iProp Σ) : iProp Σ := *)
+  (* ∃ logV logM, *)
+  (*   ⌜is_log logM logV⌝ ∗ *)
+  (*   logL ↦[ip] logV ∗ *)
+  (*   own_log_local γlog logM ∗ *)
+  (*   Res logM. *)
+
+(*
+  Lemma wp_log_wait_until ip monN monγ monV monR logL logV logM i :
+    {{{ ⌜i ≤ List.length logM⌝ ∗
+        ⌜is_log logM logV⌝ ∗
+        is_monitor monN ip monγ monV (logMonitor_res ip logL monR) ∗
+        lock_proof.locked monγ ∗ (monR logM) ∗
+        logL ↦[ip] logV }}}
+      log_wait_until #logL monV #i @[ip]
+    {{{ logV' logM', RET #();
+        ⌜i < List.length logM'⌝ ∗
+        ⌜is_log logM' logV'⌝ ∗
+        lock_proof.locked monγ ∗ (monR logM') ∗
+        logL ↦[ip] logV' }}}.
+  Proof.
+    iIntros (Φ) "(%Hi & %Hl & #Hmon & Hlocked & Hres & Hp) HΦ".
+    assert (is_log logM logV) as Hlc by done.
+    destruct Hlc as (lV & -> & Hlst).
+    wp_lam.
+    wp_pures.
+    case_bool_decide; first by lia.
+    wp_pures.
+    wp_apply (wp_log_next with "[$Hp //]").
+    iIntros (n) "(-> & %Hlc & Hp)".
+    wp_pures.
+    case_bool_decide as Hiz; first by lia.
+    wp_pure _.
+    clear Hlc.
+    iLöb as "IH" forall (logM lV Hi Hl Hlst Hiz) "Hres".
+    wp_pures.
+    wp_apply (wp_log_next with "[$Hp //]").
+    iIntros (n) "(-> & _ & Hp)".
+    wp_pures.
+    case_bool_decide as Hiz2.
+    - wp_pure _.
+      wp_apply (monitor_wait_spec with "[$Hmon Hres $Hlocked Hp]").
+      iExists _, _. iFrame. eauto.
+      iIntros (v) "(-> & Hlocked & Hres)".
+      iDestruct "Hres" as (logV' logM' Hlog') "(Hp & Hres)".
+      do 2 wp_pure _.
+      clear Hi Hl Hlst Hiz Hiz2 logM.
+      iSpecialize ("IH" $! logM' logV').
+      iApply ("IH" with "[][][][][$Hlocked][][][$Hres]").
+
+    - wp_pure _.
+      wp_apply wp_assert.
+      wp_pures.
+      iSplitR.
+      iPureIntro.
+      f_equal.
+      case_bool_decide; eauto with lia.
+      iNext.
+      iApply "HΦ".
+      iFrame.
+      eauto with lia.
+    (* -------- *)
+    iLöb as "IH".
+    wp_pures.
+    wp_apply (wp_log_next with "[$Hp //]").
+    iIntros (n) "(-> & _ & Hp)".
+    wp_pures.
+    case_bool_decide as Hiz2.
+    - wp_pure _.
+      wp_apply (monitor_wait_spec with "[$Hmon Hres $Hlocked Hp]").
+      iExists _, _. iFrame. eauto.
+      iIntros (v) "(-> & Hlocked & Hres)".
+      iDestruct "Hres" as (logV' logM' Hlog') "(Hp & Hres)".
+      do 2 wp_pure _.
+      iApply ("IH" with "[$Hlocked][Hres]").
+    - wp_pure _.
+      wp_apply wp_assert.
+      wp_pures.
+      iSplitR.
+      iPureIntro.
+      f_equal.
+      case_bool_decide; eauto with lia.
+      iNext.
+      iApply "HΦ".
+      iFrame.
+      eauto with lia.
+
+
+log_wait_until =
+(λ: "log" "mon" "i",
+   letrec: "aux" <> :=
+     let: "n" := log_next "log" in
+     if: "n" = "i" then monitor_wait "mon" ;; "aux" #()
+     else assert: "i" < "n" in
+   if: if: "i" < #0 then #true else log_next "log" < "i" then assert: #false
+   else "aux" #())%V
+     : val
+
+
+     Definition log_wait_until : val.
+
+*)
   End Log.
